working on RTac.
- ASSUMPTION now peels solved goals
  - the peeling code should be moved outward.
  - it appears that things should be relativized.
- Bug fixes to REPEAT
- Update of APPLY.
  - Now it runs a tactic as a continuation.
  - This should be generalized to support multiple goals.

examples/RTac/Demo.v
@@ -1,8 +1,21 @@
 Require Import ExtLib.Core.RelDec.
-Require Import MirrorCore.Lambda.ExprCore.
+Require Import MirrorCore.Lambda.Expr.
+Require Import MirrorCore.Lambda.ExprUnify_simul.
 Require Import MirrorCore.Lambda.Red.
-Require Import McExamples.Simple.Simple.
+Require MirrorCore.Subst.FMapSubst.
 Require Import MirrorCore.RTac.RTac.
+Require Import McExamples.Simple.Simple.
+
+Local Instance Expr_expr : Expr _ (expr typ func) := Expr_expr.
+Definition subst :=
+  FMapSubst.SUBST.raw (expr typ func).
+Local Instance Subst_subst : SubstI.Subst subst (expr typ func)
+  := FMapSubst.SUBST.Subst_subst _.
+Local Instance SubstUpdate_subst : SubstI.SubstUpdate subst (expr typ func)
+  := FMapSubst.SUBST.SubstUpdate_subst _.
+eapply instantiate.
+Defined.
+
 
 Definition open (e : expr typ func)
 : option (   ((typ * (expr typ func -> expr typ func))
@@ -15,32 +28,64 @@ Definition open (e : expr typ func)
     | _ => None
   end.
 
-Let INTRO {subst} :=
+Let INTRO :=
   INTRO (subst:=subst) (@Var typ func) open.
 
-Definition tac subst : rtac typ (expr typ func) subst :=
-  THEN (REPEAT 10 INTRO)
-       (TRY (ASSUMPTION (fun x y s => if x ?[ eq ] y then Some s else None))).
+Let APPLY := @APPLY typ (expr typ func) subst _ _ _ _
+                    (@vars_to_uvars _ _)
+                    (fun tus tvs n l r t s =>
+                       @exprUnify _ _ _ _ _ _ _ _ 10 tus tvs n s l r t)
+                    (@instantiate _ _).
+Let ASSUMPTION : rtac typ (expr typ func) subst :=
+  ASSUMPTION _ (fun x y s => if x ?[ eq ] y then Some s else None).
 
 Definition fAll (t : typ) (P : expr typ func) : expr typ func :=
   App (Inj (All t)) (Abs t P).
+
 Definition fImpl (P Q : expr typ func) : expr typ func :=
   App (App (Inj Impl) P) Q.
+
+Definition fAnd (P Q : expr typ func) : expr typ func :=
+  App (App (Inj And) P) Q.
+
+
+Definition tac : rtac typ (expr typ func) subst :=
+  THEN (REPEAT 10 INTRO)
+       (TRY ASSUMPTION).
+
 
 Definition simple_goal : expr typ func :=
   fAll tyProp (fImpl (Var 0) (Var 0)).
 
-Eval compute in fun subst (empty : subst) =>
-                  tac subst (@GGoal _ _ _ empty (Some simple_goal)).
+Definition runRTac_empty_goal (tac : rtac typ (expr typ func) subst)
+           (goal : expr typ func)  :=
+  runRTac tac (@GGoal typ (expr typ func) subst (@empty _ _ _) (Some goal)).
+
+Eval compute in
+    runRTac_empty_goal tac simple_goal.
 
 Definition simple_goal2 : expr typ func :=
   fAll tyProp (fImpl (Var 0) (fAll tyProp (Var 0))).
 
-Eval compute in fun subst (empty : subst) =>
-                  tac subst (@GGoal _ _ _ empty (Some simple_goal2)).
+Eval compute in runRTac_empty_goal tac simple_goal2.
 
 Definition simple_goal3 : expr typ func :=
   fAll tyProp (fImpl (Var 0) (fAll tyProp (Var 1))).
 
-Eval compute in fun subst (empty : subst) =>
-                  tac _ (@GGoal _ _ _ empty (Some simple_goal3)).
+Eval compute in runRTac_empty_goal tac simple_goal3.
+
+Definition and_lem : Lemma.lemma typ (expr typ func) (expr typ func) :=
+{| Lemma.vars := tyProp :: tyProp :: nil
+ ; Lemma.premises := Var 0 :: Var 1 :: nil
+ ; Lemma.concl := App (App (Inj And) (Var 0)) (Var 1)
+ |}.
+
+Eval compute in
+    let goal :=
+        fAll tyProp (fAll tyProp
+                          (fImpl (Var 0)
+                                 (fImpl (Var 1)
+                                        (fAnd (Var 0) (Var 1)))))
+    in
+    runRTac_empty_goal (THEN (REPEAT 10 INTRO)
+                             (APPLY and_lem ASSUMPTION)) goal.
