theories/RTac/Apply.v
@@ -5,9 +5,12 @@ Require Import MirrorCore.ExprI.
 Require Import MirrorCore.TypesI.
 Require Import MirrorCore.SubstI.
 Require Import MirrorCore.ExprDAs.
-Require MirrorCore.STac.Apply.
 Require Import MirrorCore.RTac.Core.
 Require Import MirrorCore.RTac.RunSTac.
+Require Import MirrorCore.Lemma.
+Require Import MirrorCore.RTac.Open.
+Require Import MirrorCore.LemmaApply.
+Require Import MirrorCore.InstantiateI.
 
 Require Import MirrorCore.Util.Forwardy.
 
@@ -28,14 +31,81 @@ Section parameterized.
   Variable SubstUpdateOk_subst : @SubstUpdateOk _ _ _ _ Expr_expr Subst_subst _ _.
 
   Variable vars_to_uvars : nat -> nat -> expr -> expr.
-  Variable exprUnify : tenv typ -> tenv typ -> nat -> expr -> expr -> typ -> subst -> option subst.
+  Variable exprUnify :
+    tenv typ -> tenv typ -> nat -> expr -> expr -> typ -> subst -> option subst.
   Variable instantiate : (nat -> option expr) -> nat -> expr -> expr.
 
-  Definition APPLY (l : Lemma.lemma typ expr expr)
-             (ctac : Continuation.stac_cont typ expr subst)
+  Let eapplicable :=
+    @eapplicable typ _ expr _ subst vars_to_uvars
+                 exprUnify.
+
+  Section fm2.
+    Variable T U V : Type.
+    Variable f : T -> U -> option V.
+    Fixpoint filter_map2 (ls : list T) (ls' : list U) : option (list V) :=
+      match ls , ls' with
+        | nil , nil => Some nil
+        | l :: ls , l' :: ls' =>
+          match f l l' with
+            | None => filter_map2 ls ls'
+            | Some x => match filter_map2 ls ls' with
+                          | None => None
+                          | Some xs => Some (x :: xs)
+                        end
+          end
+        | _ , _ => None
+      end.
+  End fm2.
+
+  Fixpoint all_success (f : expr -> subst -> option (Goal typ expr subst))
+           (sub : _) (ls : list expr)
+  : option (Goal typ expr subst) :=
+    match ls with
+      | nil => Some (GGoal sub None)
+      | l :: ls =>
+        match f l sub with
+          | None => None
+          | Some (GGoal sub' None) => all_success f sub' ls
+          | Some x =>
+            match ls with
+              | nil => Some x
+              | _ :: _ => None
+            end
+        end
+    end.
+
+  Definition APPLY
+             (lem : Lemma.lemma typ expr expr)
+             (ctac : rtac typ expr subst)
   : rtac typ expr subst :=
-    STAC_no_hyps
-      (@Apply.APPLY typ expr subst _ _ vars_to_uvars exprUnify instantiate
-                    _ _ l ctac).
+    let len_vars := length lem.(vars) in
+    fun gl =>
+      let '(ctx,sub,goal) := openGoal gl in
+      match goal with
+        | None => Some gl
+        | Some goal =>
+          let '(tus,tvs) := getEnvs ctx in
+          match eapplicable sub tus tvs lem goal with
+            | None => None
+            | Some sub' =>
+              let len_uvars := length tus in
+              match pull (expr := expr) (SU := SU) len_uvars len_vars sub' with
+                | Some sub'' =>
+                  let premises :=
+                      map (fun e => instantiate (fun u => lookup u sub') 0
+                                                (vars_to_uvars 0 len_uvars e))
+                          lem.(premises)
+                  in
+                  (** Solve the side conditions **)
+                  all_success
+                    (fun goal_expression sub =>
+                       let goal := closeGoal ctx (GGoal sub (Some goal_expression)) in
+                       ctac goal)
+                    sub''
+                    premises
+                | None => None
+              end
+          end
+      end.
 
 End parameterized.
