theories/RTac/Assumption.v
@@ -22,7 +22,8 @@ Section parameterized.
   Variable Typ0_Prop : Typ0 _ Prop.
   Variable Subst_subst : Subst subst expr.
   Variable SubstOk_subst : @SubstOk _ _ _ _ Expr_expr Subst_subst.
-
+  Variable SubstUpdate_subst : SubstUpdate subst expr.
+  Variable SubstUpdateOk_subst : @SubstUpdateOk _ _ _ _ Expr_expr Subst_subst _ _.
 
   Variable (check : expr -> expr -> subst -> option subst).
 
@@ -38,15 +39,47 @@ Section parameterized.
                        end
     end.
 
+  Fixpoint reduceGoal (ctx : Ctx typ expr) (s : subst) (un vn : nat)
+  : Ctx typ expr * subst :=
+    match ctx with
+      | CTop => (ctx, s)
+      | CAll l ctx' =>
+        match vn with
+          | 0 => (** STUCK **)
+            (ctx, s)
+          | S vn' =>
+            (** TODO: Drop var **)
+            reduceGoal ctx' s un vn'
+        end
+      | CEx  l ctx' =>
+        match un with
+          | 0 => (** STUCK **)
+            (ctx, s)
+          | S un' =>
+            match drop un' s with
+              | Some s' =>
+                reduceGoal ctx' s' un' vn
+              | None => (** STUCK **)
+                (ctx, s)
+            end
+        end
+      | CHyp h ctx' =>
+        reduceGoal ctx' s un vn
+    end.
+
   Definition ASSUMPTION : rtac typ (expr) subst :=
     fun g =>
       let '(ctx,s,gl) := openGoal g in
       match gl with
         | None => Some g
-        | Some gl => match findHyp s ctx gl with
-                       | None => None
-                       | Some s => Some (closeGoal ctx (GGoal s None))
-                     end
+        | Some gl =>
+          match findHyp s ctx gl with
+            | None => None
+            | Some s' =>
+              let (tus,tvs) := getEnvs ctx in
+              let (ctx',s'') := reduceGoal ctx s' (length tus) (length tvs) in
+              Some (closeGoal ctx' (GGoal s'' None))
+          end
       end.
 
   (** check soundness **)
